Use binding_list and structure for env

src/env/defs.lean
@@ -1,69 +1,58 @@
-import sch
+import .binding_list
 
 namespace tts ------------------------------------------------------------------
 
--- An environment is an association list of type bindings or pairs of a variable
--- and the variable's type scheme.
-@[inline, reducible]
-def env (V : Type) : Type :=
-  list (V × sch V)
+-- An environment is list of variable-type scheme bindings.
+structure env (V : Type) : Type :=
+  (bindings : list (binding V))
 
 variables {V : Type} -- Type of variable names
 
+-- These are definitions on the environment. Some of them wrap the binding_list
+-- definitions.
 namespace env ------------------------------------------------------------------
 
-@[pattern, inline, reducible]
-def binding : V → sch V → V × sch V :=
-  prod.mk
-
--- A binding appears somewhere in the environment
-def binds (x : V) (s : sch V) (Γ : env V) : Prop :=
-  binding x s ∈ Γ
-
--- A singleton environment
-def one (x : V) (s : sch V) : env V :=
-  [binding x s]
+-- An empty environment
+instance : has_emptyc (env V) :=
+  ⟨⟨list.nil⟩⟩
 
 -- Add a binding to an environment
-def add (x : V) (s : sch V) (Γ : env V) : env V :=
-   one x s ++ Γ
+instance has_insert : has_insert (binding V) (env V) :=
+  ⟨λ b ⟨Γ⟩, ⟨b :: Γ⟩⟩
 
--- All of the remaining definitions require decidable equality on V
+-- A singleton environment
+def one (b : binding V) : env V :=
+  ⟨[b]⟩
+
+-- A binding appears somewhere in the environment
+instance has_mem : has_mem (binding V) (env V) :=
+  ⟨λ b ⟨Γ⟩, b ∈ Γ⟩
+
+-- Append one environment to another
+instance has_append : has_append (env V) :=
+  ⟨λ ⟨Γ₁⟩ ⟨Γ₂⟩, ⟨Γ₁ ++ Γ₂⟩⟩
+
+-- Map a function over the type scheme of an environment
+def map (f : sch V → sch V) : env V → env V
+  | ⟨Γ⟩ := ⟨Γ.map (binding.map f)⟩
+
 variables [decidable_eq V]
 
 -- Free variables of an environment
 def fv : env V → finset V
-  | []                 := ∅
-  | (binding _ s :: Γ) := s.fv ∪ fv Γ
+  | ⟨Γ⟩ := binding_list.fv Γ
 
 -- Domain of an environment
 def dom : env V → finset V
-  | []                 := ∅
-  | (binding v _ :: Γ) := insert v (dom Γ)
-
--- Domain of an environment
-@[inline, reducible]
-def map (f : sch V → sch V) : env V → env V :=
-  list.map (prod.map id f)
-
--- A variable is not bound in the environment
-@[inline, reducible]
-def unbound (x : V) (Γ : env V) : Prop :=
-  x ∉ dom Γ
-
--- If every variable is bound only once in the environment
-inductive uniq : env V → Prop
-  | empty : uniq []
-  | push  : Π (x : V) (s : sch V) (Γ : env V), Γ.unbound x → uniq Γ → uniq (Γ.add x s)
+  | ⟨Γ⟩ := binding_list.dom Γ
 
 -- When the domains of two environments are disjoint
-def disjoint (Γ₁ : env V) (Γ₂ : env V) : Prop :=
-  dom Γ₁ ∩ dom Γ₂ = ∅
+def disjoint : env V → env V → Prop
+  | ⟨Γ₁⟩ ⟨Γ₂⟩ := binding_list.disjoint Γ₁ Γ₂
 
--- Get the first type scheme bound to the variable x
-def get (x : V) : env V → option (sch V)
-  | []                 := none
-  | (binding y s :: t) := if h : y = x then some s else get t
+-- If every variable is bound only once in the environment
+def uniq : env V → Prop
+  | ⟨Γ⟩ := binding_list.uniq Γ
 
 end /- namespace -/ env --------------------------------------------------------
 end /- namespace -/ tts --------------------------------------------------------
