src/env/binding_list/binding.lean
@@ -1,0 +1,22 @@
+import sch
+
+namespace tts ------------------------------------------------------------------
+
+-- A pair of a variable and a type scheme.
+structure binding (V : Type) : Type :=
+  (var : V)
+  (sch : sch V)
+
+infix ` :~ `:80 := binding.mk
+
+variables {V : Type} -- Type of variable names
+
+namespace binding --------------------------------------------------------------
+
+-- Map a function over the type scheme of a binding.
+protected
+def map (f : tts.sch V → tts.sch V) : binding V → binding V
+  | (binding.mk x s) := binding.mk x (f s)
+
+end /- namespace -/ binding ----------------------------------------------------
+end /- namespace -/ tts --------------------------------------------------------
