src/env/binding_list/defs.lean
@@ -1,0 +1,30 @@
+-- These are definitions on the underlying list of bindings.
+
+import .binding
+
+namespace tts ------------------------------------------------------------------
+namespace binding_list ---------------------------------------------------------
+
+variables {V : Type} [decidable_eq V] -- Type of variable names
+
+-- Free variables of a binding list
+def fv : list (binding V) → finset V
+  | []            := ∅
+  | (x :~ s :: Γ) := s.fv ∪ fv Γ
+
+-- Domain of a binding list
+def dom : list (binding V) → finset V
+  | []            := ∅
+  | (x :~ _ :: Γ) := insert x (dom Γ)
+
+-- When the domains of two binding lists are disjoint
+def disjoint (Γ₁ : list (binding V)) (Γ₂ : list (binding V)) : Prop :=
+  dom Γ₁ ∩ dom Γ₂ = ∅
+
+-- If every variable is bound only once in the binding list
+inductive uniq : list (binding V) → Prop
+  | nil  :                                                                    uniq []
+  | cons : Π {b : binding V} {Γ : list (binding V)}, b.var ∉ dom Γ → uniq Γ → uniq (b :: Γ)
+
+end /- namespace -/ binding_list -----------------------------------------------
+end /- namespace -/ tts --------------------------------------------------------
