src/env/binding_list/props.lean
@@ -1,0 +1,311 @@
+import .defs
+import data.multiset.extra
+import logic.basic
+
+open function
+
+namespace tts ------------------------------------------------------------------
+namespace binding_list ---------------------------------------------------------
+
+variables {V : Type} -- Type of variable names
+variables {x x₁ x₂ : V} -- Variables
+variables {s s₁ s₂ : sch V} -- Type schemes
+variables {fs : sch V → sch V} -- Type scheme function
+variables {b : binding V} -- Bindings
+variables {Γ Γ₁ Γ₂ Γ₃ : list (binding V)} -- Binding lists
+
+-- Use notation to avoid ambiguity.
+local notation `[]` := (list.nil : list (binding V))
+local notation h :: t  := (list.cons h (t : list (binding V)) : list (binding V))
+
+-- Keep and-chains right-associated
+local attribute [simp] and.assoc
+
+-- Conjunctive normal form
+local attribute [simp] decidable.not_or_iff_and_not
+
+@[inline, reducible, simp]
+private
+def map (fs : sch V → sch V) : list (binding V) → list (binding V) :=
+  list.map (binding.map fs)
+
+-- Basic properties of binding
+section binding ----------------------------------------------------------------
+
+@[simp]
+theorem binding_var : (x :~ s).var = x :=
+  rfl
+
+@[simp]
+theorem binding_sch : (x :~ s).sch = s :=
+  rfl
+
+@[simp]
+theorem binding_map : binding.map fs (x :~ s) = x :~ fs s :=
+  rfl
+
+theorem binding_map_inj (fs_inj : injective fs) : injective (binding.map fs) :=
+  λ ⟨x₁, s₁⟩ ⟨x₂, s₂⟩ h,
+  begin
+    injection h with h_x h_fs_s,
+    have h_s : s₁ = s₂ := fs_inj h_fs_s,
+    subst h_x,
+    subst h_s
+  end
+
+end /- section -/ binding ------------------------------------------------------
+
+-- Basic properties of mem and map
+section mem_map ----------------------------------------------------------------
+
+@[simp]
+theorem map_cons : map fs (b :: Γ) = b.var :~ fs b.sch :: map fs Γ :=
+  by cases b; refl
+
+end /- section -/ mem_map ------------------------------------------------------
+
+-- Basic properties of dom
+section dom --------------------------------------------------------------------
+variables [decidable_eq V]
+local attribute [simp] dom
+
+@[simp]
+theorem dom_nil : dom [] = (∅ : finset V) :=
+  rfl
+
+@[simp]
+theorem dom_one : dom [x :~ s] = finset.singleton x :=
+  rfl
+
+@[simp]
+theorem dom_cons_val : (dom (x :~ s :: Γ)).val = multiset.ndinsert x ((dom Γ).val) :=
+  begin
+    cases Γ,
+    case list.nil { simp },
+    case list.cons : hd tl { cases hd, simp }
+  end
+
+@[simp]
+theorem dom_cons_insert : dom (b :: Γ) = insert b.var (dom Γ) :=
+  by cases b; simp
+
+@[simp]
+theorem dom_append : dom (Γ₁ ++ Γ₂) = dom Γ₁ ∪ dom Γ₂ :=
+  by induction Γ₁ with _ _ ih; simp; simp [ih]
+
+@[simp]
+theorem dom_map : dom (map fs Γ) = dom Γ :=
+  by induction Γ with _ _ ih; simp; simp [ih]
+
+@[simp]
+theorem mem_dom_wrap : x ∈ (dom Γ).val ↔ x ∈ dom Γ :=
+  by induction Γ with hd tl ih; [simp, {cases hd, simp [ih]}]
+
+@[simp]
+theorem mem_dom_nil : x ∈ dom [] ↔ false :=
+  by refl
+
+@[simp]
+theorem not_mem_dom_map : x ∉ dom (map fs Γ) ↔ x ∉ dom Γ :=
+  by simp
+
+end /- section -/ dom ----------------------------------------------------------
+
+-- Basic properties of disjoint
+section disjoint ---------------------------------------------------------------
+variables [decidable_eq V]
+
+theorem disjoint_multiset : disjoint Γ₁ Γ₂ ↔ multiset.disjoint (dom Γ₁).val (dom Γ₂).val :=
+  finset.inter_eq_empty_iff_disjoint
+
+-- We reuse the multiset simplifier theorems in this section.
+local attribute [simp] disjoint_multiset
+
+theorem disjoint.symm : disjoint Γ₁ Γ₂ → disjoint Γ₂ Γ₁ :=
+  by simp
+
+theorem disjoint_comm : disjoint Γ₁ Γ₂ ↔ disjoint Γ₂ Γ₁ :=
+  by simp
+
+@[simp]
+theorem disjoint_nil : disjoint [] Γ ↔ true :=
+  iff_true_intro (by simp)
+
+@[simp]
+theorem disjoint_one : disjoint [x :~ s] Γ ↔ x ∉ dom Γ :=
+  by simp
+
+private
+lemma not_mem_dom_of_disjoint_cons : disjoint (b :: Γ₁) Γ₂ → b.var ∉ dom Γ₂ :=
+  by intro h; simp at h; exact h.1
+
+private
+lemma disjoint_of_disjoint_cons : disjoint (b :: Γ₁) Γ₂ → disjoint Γ₁ Γ₂ :=
+  by simp
+
+private
+lemma disjoint_cons : b.var ∉ dom Γ₂ → disjoint Γ₁ Γ₂ → disjoint (b :: Γ₁) Γ₂ :=
+  by simp; exact and.intro
+
+@[simp]
+theorem disjoint_cons : disjoint (b :: Γ₁) Γ₂ ↔ b.var ∉ dom Γ₂ ∧ disjoint Γ₁ Γ₂ :=
+  ⟨ λ h, ⟨not_mem_dom_of_disjoint_cons h, disjoint_of_disjoint_cons h⟩
+  , λ h, disjoint_cons h.1 h.2
+  ⟩
+
+@[simp]
+theorem disjoint_append : disjoint (Γ₁ ++ Γ₂) Γ₃ ↔ disjoint Γ₁ Γ₃ ∧ disjoint Γ₂ Γ₃ :=
+  by simp
+
+@[simp]
+theorem disjoint_map : disjoint (map fs Γ₁) Γ₂ ↔ disjoint Γ₁ Γ₂ :=
+  by simp
+
+end /- section -/ disjoint -----------------------------------------------------
+
+-- Basic properties of uniq
+section uniq -------------------------------------------------------------------
+variables [decidable_eq V]
+
+@[simp]
+theorem uniq_empty : uniq [] ↔ true :=
+  iff_true_intro uniq.nil
+
+@[simp]
+theorem uniq_one : uniq [b] ↔ true :=
+  iff_true_intro (uniq.cons mem_dom_nil.mp uniq.nil)
+
+@[simp]
+theorem uniq_cons : uniq (b :: Γ) ↔ b.var ∉ dom Γ ∧ uniq Γ :=
+  ⟨λ u, by cases u with _ _ hd tl; exact ⟨hd, tl⟩, λ ⟨hd, tl⟩, uniq.cons hd tl⟩
+
+private
+lemma uniq_append_left : uniq (Γ₁ ++ Γ₂) → uniq Γ₁ ∧ uniq Γ₂ ∧ disjoint Γ₁ Γ₂ :=
+  begin
+    induction Γ₁ with hd tl ih; [simp, {cases hd, simp}],
+    intros ub₁ ub₂ u,
+    have p : uniq tl ∧ uniq Γ₂ ∧ disjoint tl Γ₂ := ih u,
+    exact ⟨ub₂, ⟨p.1, ⟨p.2.1, ⟨ub₁, p.2.2⟩⟩⟩⟩
+  end
+
+private
+lemma uniq_append_right : uniq Γ₁ ∧ uniq Γ₂ ∧ disjoint Γ₁ Γ₂ → uniq (Γ₁ ++ Γ₂) :=
+  begin
+    induction Γ₁ with hd tl ih; [simp, {cases hd, simp [ih]}],
+    intros ub_tl un_tl un_Γ₂ ub_Γ₂ d_tl_Γ₂,
+    exact ⟨ub_Γ₂, ⟨ub_tl, ih ⟨un_tl, un_Γ₂, d_tl_Γ₂⟩⟩⟩
+  end
+
+@[simp]
+theorem uniq_append : uniq (Γ₁ ++ Γ₂) ↔ uniq Γ₁ ∧ uniq Γ₂ ∧ disjoint Γ₁ Γ₂ :=
+  ⟨uniq_append_left, uniq_append_right⟩
+
+@[simp]
+theorem uniq_map : uniq (map fs Γ) ↔ uniq Γ :=
+  by induction Γ with hd tl ih; [simp, {cases hd, simp [ih]}]
+
+end /- section -/ uniq ---------------------------------------------------------
+
+-- More properties of mem
+section mem --------------------------------------------------------------------
+
+private
+lemma mem_map_of_inj' (h : injective (binding.map fs))
+: binding.map fs (x :~ s) ∈ list.map (binding.map fs) Γ ↔ x :~ s ∈ Γ :=
+  list.mem_map_of_inj h
+
+theorem mem_map_of_inj (h : injective fs)
+: x :~ fs s ∈ map fs Γ ↔ x :~ s ∈ Γ :=
+  mem_map_of_inj' (binding_map_inj h)
+
+theorem mem_map : x :~ s₁ ∈ map fs Γ ↔ ∃ s₂, x :~ s₂ ∈ Γ ∧ fs s₂ = s₁ :=
+  begin
+    split,
+    begin
+      intro h,
+      rcases list.mem_map.mp h with ⟨b, h₁, h₂⟩,
+      cases b with x₂ s₂,
+      injection h₂ with h_x h_fs_s,
+      subst h_x,
+      exact ⟨s₂, ⟨h₁, h_fs_s⟩⟩
+    end,
+    begin
+      intro h,
+      rcases h with ⟨s₂, h₁, h₂⟩,
+      exact list.mem_map.mpr ⟨x :~ s₂, ⟨h₁, by rw [binding.map, h₂]⟩⟩
+    end
+  end
+
+private
+lemma mem_map_of_mem'
+: x :~ s ∈ Γ → binding.map fs (x :~ s) ∈ list.map (binding.map fs) Γ :=
+  list.mem_map_of_mem (binding.map fs)
+
+theorem mem_map_of_mem : x :~ s ∈ Γ → x :~ fs s ∈ map fs Γ :=
+  mem_map_of_mem'
+
+variables [decidable_eq V]
+
+theorem mem_dom_of_mem : x :~ s ∈ Γ → x ∈ dom Γ :=
+  begin
+    induction Γ with hd tl ih; [simp, {cases hd, simp}],
+    exact or.imp and.left ih
+  end
+
+private
+lemma disjoint_forall₁ : disjoint Γ₁ Γ₂ → ∀ {b : binding V}, b ∈ Γ₁ → b.var ∉ dom Γ₂ :=
+  begin
+    induction Γ₁ with hd tl ih; [simp, {cases hd, simp}],
+    exact λ ub d, ⟨ub, λ b h, ih d h⟩
+  end
+
+private
+lemma disjoint_forall₂ : (∀ {b : binding V}, b ∈ Γ₁ → b.var ∉ dom Γ₂) → disjoint Γ₁ Γ₂ :=
+  begin
+    induction Γ₁ with hd tl ih; [simp, {cases hd, simp}],
+    exact λ ub f, ⟨ub, ih f⟩
+  end
+
+theorem disjoint_forall : disjoint Γ₁ Γ₂ ↔ ∀ {b : binding V}, b ∈ Γ₁ → b.var ∉ dom Γ₂ :=
+  ⟨disjoint_forall₁, disjoint_forall₂⟩
+
+private
+lemma mem_cons_of_uniq_cons'
+: uniq (x₂ :~ s₂ :: Γ)
+→ x₁ :~ s₁ ∈ x₂ :~ s₂ :: Γ
+→ x₁ = x₂ ∧ s₁ = s₂ ∧ x₁ ∉ dom Γ ∨ x₁ :~ s₁ ∈ Γ ∧ x₁ ≠ x₂ :=
+  begin
+    simp,
+    intros b u h,
+    exact match h with
+      | or.inl ⟨h₁, h₂⟩ := or.inl ⟨h₁, ⟨h₂, eq.rec_on h₁.symm b⟩⟩
+      | or.inr h        := or.inr ⟨h, ne_of_mem_of_not_mem (mem_dom_of_mem h) b⟩
+    end
+  end
+
+theorem mem_cons_of_uniq_cons
+: uniq (x₂ :~ s₂ :: Γ)
+→ (x₁ :~ s₁ ∈ x₂ :~ s₂ :: Γ ↔ x₁ = x₂ ∧ s₁ = s₂ ∧ x₁ ∉ dom Γ ∨ x₁ :~ s₁ ∈ Γ ∧ x₁ ≠ x₂) :=
+  λ u, ⟨mem_cons_of_uniq_cons' u, by simp; exact or.imp (λ h, ⟨h.1, h.2.1⟩) and.left⟩
+
+private
+lemma mem_append_of_uniq_append'
+: uniq (Γ₁ ++ Γ₂)
+→ x :~ s ∈ Γ₁ ++ Γ₂
+→ x :~ s ∈ Γ₁ ∧ x ∉ dom Γ₂ ∨ x ∉ dom Γ₁ ∧ x :~ s ∈ Γ₂ :=
+  begin
+    simp,
+    intros _ _ d,
+    exact or.imp (λ b, ⟨b, disjoint_forall.mp d b⟩)
+                 (λ b, ⟨disjoint_forall.mp d.symm b, b⟩)
+  end
+
+theorem mem_append_of_uniq_append
+: uniq (Γ₁ ++ Γ₂)
+→ (x :~ s ∈ Γ₁ ++ Γ₂ ↔ x :~ s ∈ Γ₁ ∧ x ∉ dom Γ₂ ∨ x ∉ dom Γ₁ ∧ x :~ s ∈ Γ₂) :=
+  λ u, ⟨mem_append_of_uniq_append' u, list.mem_append.mpr ∘ or.imp and.left and.right⟩
+
+end /- section -/ mem ----------------------------------------------------------
+
+end /- namespace -/ binding_list -----------------------------------------------
+end /- namespace -/ tts --------------------------------------------------------
