src/typing.lean
@@ -2,29 +2,29 @@ import .env
 import .exp
 
 namespace tts ------------------------------------------------------------------
-variables {V : Type} [decidable_eq V] [finset.has_fresh V] -- Type of variable names
+variables {V : Type} [decidable_eq V] -- Type of variable names
 
 open exp
 open typ
 
 inductive typing : env V → exp V → typ V → Prop
   | varf : Π {Γ : env V} {x : V} {s : sch V} {ts : list (typ V)}
-     , Γ.uniq
-     → Γ.binds x s
-     → lc_types s.arity ts
-     → s.well_formed
-     → typing Γ (varf x) (s.open ts)
+    , Γ.uniq
+    → x :~ s ∈ Γ
+    → lc_types s.arity ts
+    → s.well_formed
+    → typing Γ (varf x) (s.open ts)
   | app : Π {Γ : env V} {ef ea : exp V} {t₁ t₂ : typ V}
-      , typing Γ ef (arr t₁ t₂)
-      → typing Γ ea t₁
-      → typing Γ (app ef ea) t₂
+    , typing Γ ef (arr t₁ t₂)
+    → typing Γ ea t₁
+    → typing Γ (app ef ea) t₂
   | lam : Π {L : finset V} {Γ : env V} {e : exp V} {t₁ t₂ : typ V}
-      , t₁.lc
-      → (∀ x : V, x ∉ L → typing (Γ.add x ⟨0, t₁⟩) (e.open_var x) t₂)
-      → typing Γ (lam e) (arr t₁ t₂)
+    , t₁.lc
+    → (∀ x : V, x ∉ L → typing (insert ⟨x, ⟨0, t₁⟩⟩ Γ) (e.open_var x) t₂)
+    → typing Γ (lam e) (arr t₁ t₂)
   | let_ : Π {L₁ L₂ : finset V} {Γ : env V} {e₁ e₂ : exp V} {s₁ : sch V} {t₂ : typ V}
-      , (∀ xs : list V, fresh L₁ s₁.arity xs → typing Γ e₁ (s₁.open_vars xs))
-      → (∀ x : V, x ∉ L₂ → typing (Γ.add x s₁) (e₂.open_var x) t₂)
-      → typing Γ (let_ e₁ e₂) t₂
+    , (∀ xs : list V, fresh L₁ s₁.arity xs → typing Γ e₁ (s₁.open_vars xs))
+    → (∀ x : V, x ∉ L₂ → typing (insert ⟨x, s₁⟩ Γ) (e₂.open_var x) t₂)
+    → typing Γ (let_ e₁ e₂) t₂
 
 end /- namespace -/ tts --------------------------------------------------------
